working on axiomatic semantics

concurrency/Machine_ax.v
@@ -1,15 +1,94 @@
 Require Import concurrency.Asm_core. (* for AxiomaticCoreSem.
                             TODO: Move it out of there and
                             stop importing Asm_core *)
+Import AxCoreSem.
 
-(* Module Type Semantics. *)
-(*   Parameter G: Type. *)
-(*   Parameter C: Type. *)
-(*   Parameter Sem: @AxiomaticCoreSem G C. *)
-(*   (* Parameter getEnv : G -> Genv.t F V. *) *)
-(* End Semantics. *)
+Module Type Semantics.
+  Parameter G: Type.
+  Parameter C: Type.
+  Parameter E:Type.
+  Parameter Sem: @AxiomaticCoreSemantics G C E.
+End Semantics.
 
-(* Module Type ThreadPool. *)
+Module Type ThreadPoolSig.
+  Declare Module SEM: Semantics.
+
+  Definition tid := nat.
+  Parameter t : Type.
+
+  Parameter getThread: tid -> t -> option SEM.C.
+  Parameter updThread: tid -> SEM.C -> t -> t.
+  Parameter gsoThread:
+    forall i j t c (Hneq: i <> j),
+      getThread i (updThread j c t) = getThread i t.
+  Parameter gssThread:
+    forall i t c,
+      getThread i (updThread i c t) = Some c.
+End ThreadPoolSig.
+
+Module ThreadPool <: ThreadPoolSig.
+
+  Declare Module SEM:Semantics.
+  Definition tid := nat.
+  Definition t := tid -> option SEM.C.
+
+  Definition getThread i (tp: t) := tp i.
+  Definition updThread i c (tp : t) :=
+    fun j => if (PeanoNat.Nat.eq_dec i j) then Some c else tp j.
+
+  Lemma gsoThread:
+    forall i j t c (Hneq: i <> j),
+      getThread i (updThread j c t) = getThread i t.
+  Proof.
+    intros.
+    unfold getThread, updThread.
+    destruct eq_dec.EqDec_nat; subst;
+      [exfalso|]; now auto.
+  Qed.
+
+  Lemma gssThread:
+    forall i t c,
+      getThread i (updThread i c t) = Some c.
+  Proof.
+    intros.
+    unfold getThread, updThread.
+    destruct (PeanoNat.Nat.eq_dec i i); now tauto.
+  Qed.
+End ThreadPool.
+
+Module Type AxMachine (SEM:Semantics)
+       (ThreadPool : ThreadPoolSig with Module SEM := SEM).
+  Import ThreadPool SEM.
+
+  Notation tstep := (corestep G C E Sem).
+
+  (** Parameterized over external (concurrent) steps*)
+  Parameter cstep: G -> t -> tid -> list E -> t -> Prop.
+
+  Inductive step {genv:G} (tp : t) (i: tid): list E -> t -> Prop :=
+  | InternalStep:
+      forall c c' evl
+        (Hget: getThread i tp = Some c)
+        (Hstep: tstep genv c c' evl),
+        step tp i evl (updThread i c' tp)
+  | ExternalStep:
+      forall  evl tp'
+         (Hcstep: cstep genv tp i evl tp'),
+        step tp i evl tp'.
+
+End AxMachine.
+
+Module AxLockMachine (SEM:Semantics)
+       (ThreadPool : ThreadPoolSig with Module SEM := SEM) <:
+  AxMachine SEM ThreadPool.
+  Import ThreadPool SEM.
+
+  Parameter lockE: list E.
+  Parameter unlockE: list E.
+  Parameter 
+
+  Inductive cstep {genv:G} (tp : t) (i : tid): list E
+    
 
 
-(* Definition threadPool : Type := fun nat =>  *)
+
